semantics/proofs/evaluatePropsScript.sml
@@ -4,7 +4,8 @@
 
 open preamble evaluateTheory
      namespaceTheory namespacePropsTheory
-     semanticPrimitivesTheory semanticPrimitivesPropsTheory;
+     semanticPrimitivesTheory semanticPrimitivesPropsTheory
+     fpSemPropsTheory;
 open terminationTheory
 
 val _ = new_theory"evaluateProps";
@@ -100,6 +101,7 @@ Proof
   ho_match_mp_tac terminationTheory.evaluate_ind >>
   srw_tac[][terminationTheory.evaluate_def] >>
   every_case_tac >> full_simp_tac(srw_ss())[] >>
+  fs[shift_fp_opts_def] >>
   TRY (
     rename1`op ≠ Opapp` >> fs[] >>
     imp_res_tac do_app_call_FFI_rel >>
@@ -298,26 +300,27 @@ Theorem is_clock_io_mono_do_app:
    is_clock_io_mono (\st'. case do_app (st'.refs, st'.ffi) op xs of
       NONE => (st', Rerr (Rabort Rtype_error))
     | SOME ((refs,ffi),r) =>
-      if (isFpOp op)
-      then
-        let
-          fp_opt =
-            (case (do_fprw r (st'.fp_opts (App op es)) (st'.fp_rws)) of
-            (* if it fails, just use the old value tree *)
-              NONE => r
-            | SOME r_opt => r_opt)
-          in
-          let fp_res =
-            (if (isFpBool op)
-            then (case fp_opt of
-                Rval (ValueTree fv) => compress fv
-              | _ => Rerr (Rabort Rtype_error)
-              )
-            else fp_opt)
-        in ( st' with<| refs := refs; ffi := ffi |>, list_result fp_res)
+      if isFpOp op then
+        (let
+           fp_opt =
+             case
+               do_fprw r (st'.fp_opts 0) st'.fp_rws
+             of
+               NONE => r
+             | SOME r_opt => r_opt ;
+           fp_res =
+             if isFpBool op then
+               case fp_opt of
+               Rval (FP_BoolTree fv) =>
+                   Rval (Boolv (compress_bool fv))
+               | _ => (Rerr (Rabort Rtype_error))
+             else fp_opt
+         in
+           (shift_fp_opts (st' with <|refs := refs; ffi := ffi|>),
+            list_result fp_res))
       else (st' with<| refs := refs; ffi := ffi |>, list_result r)) st
 Proof
-  fs [is_clock_io_mono_def]
+  fs [is_clock_io_mono_def, shift_fp_opts_def]
   \\ rpt (CASE_TAC ORELSE CHANGED_TAC (fs []) ORELSE strip_tac)
   \\ metis_tac [do_app_io_events_mono]
 QED
@@ -481,7 +484,8 @@ Proof
  >> Cases_on `r`
  >> simp []
  >> drule evaluate_sing
- >> rw [] \\ rw[]);
+ >> rw [] >> rw[]
+QED
 
 Theorem evaluate_decs_nil[simp]:
    ∀(s:'ffi state) env.
@@ -738,7 +742,7 @@ Proof
  >> rw [evaluate_def]
  >> every_case_tac
  >> fs []
- >> rw [dec_clock_def]
+ >> rw [dec_clock_def, shift_fp_opts_def]
 QED
 
  (*
@@ -787,36 +791,6 @@ val option_CASE_fst_cong = Q.prove(
 
 val evaluate_state_const = CONJUNCT1 evaluate_state_unchanged;
 
-Theorem evaluate_fp_opts_unchanged :
-  (! (s:'a state) env e s' r.
-    evaluate s env e = (s', r) ==>
-    s.fp_opts = s'.fp_opts /\
-    s.fp_rws = s'.fp_rws) /\
-  (! (s:'a state) env v pes errv s' r.
-    evaluate_match s env v pes errv = (s', r) ==>
-    s.fp_opts = s'.fp_opts /\
-    s.fp_rws = s'.fp_rws)
-Proof
-  ho_match_mp_tac evaluate_ind \\ rw[]
-  \\ rfs[evaluate_def]
-  \\ qpat_x_assum `_ = (_,_)` mp_tac
-  \\ rpt (TOP_CASE_TAC \\ fs[])
-  \\ rpt strip_tac \\ rveq
-  \\ res_tac \\ fs[dec_clock_def]
-QED
-
-Theorem fpOp_determ:
-  ! op refs refsN (ffi1 ffi1':'a ffi_state) (ffi2:'b ffi_state) r vl.
-    isFpOp op /\
-    do_app (refs, ffi1) op vl = SOME ((refsN, ffi1'), r) ==>
-    do_app (refs, ffi2) op vl = SOME ((refsN, ffi2), r)
-Proof
-  rpt strip_tac \\ Cases_on `op` \\ fs[astTheory.isFpOp_def]
-  \\ rpt (qpat_x_assum `do_app _ _ _ = _` mp_tac)
-  \\ fs[do_app_def]
-  \\ rpt (TOP_CASE_TAC \\ fs[])
-QED
-
 Theorem evaluate_ffi_intro:
     (∀(s:'a state) env e s' r.
      evaluate s env e = (s',r) ∧
@@ -827,7 +801,7 @@ Theorem evaluate_ffi_intro:
        t.clock = s.clock ∧ t.refs = s.refs /\
        t.fp_opts = s.fp_opts /\ t.fp_rws = s.fp_rws
        ⇒
-       evaluate t env e = (t with <| clock := s'.clock; refs := s'.refs |>, r)) ∧
+       evaluate t env e = (t with <| clock := s'.clock; refs := s'.refs; fp_opts := s'.fp_opts |>, r)) ∧
   (∀(s:'a state) env v pes errv s' r.
      evaluate_match s env v pes errv = (s',r) ∧
      s'.ffi = s.ffi ∧
@@ -837,7 +811,7 @@ Theorem evaluate_ffi_intro:
        t.clock = s.clock ∧ t.refs = s.refs /\
        t.fp_opts = s.fp_opts /\ t.fp_rws = s.fp_rws
        ⇒
-       evaluate_match t env v pes errv = (t with <| clock := s'.clock; refs := s'.refs |>, r))
+       evaluate_match t env v pes errv = (t with <| clock := s'.clock; refs := s'.refs; fp_opts := s'.fp_opts |>, r))
 Proof
   ho_match_mp_tac evaluate_ind
   \\ rw[]
@@ -860,8 +834,9 @@ Proof
     \\ imp_res_tac evaluate_state_const \\ fs[]
     \\ every_case_tac >> rfs[]
     \\ res_tac
-    \\ imp_res_tac evaluate_fp_opts_unchanged
-    \\ first_x_assum (qspec_then `t1` mp_tac) \\ rveq \\ fs[])
+    \\ imp_res_tac evaluate_fp_opts_fixed
+    \\ first_x_assum (qspec_then `t1` mp_tac) \\ rveq \\ fs[]
+    \\ disch_then irule)
   >- (
     rfs[evaluate_def] \\ rw[state_component_equality] )
   >- (
@@ -882,7 +857,7 @@ Proof
     \\ fs[] \\ rfs[]
     \\ qmatch_goalsub_abbrev_tac`evaluate_match t1`
     \\ first_x_assum (qspec_then `t1` mp_tac) \\ fs[Abbr`t1`]
-    \\ imp_res_tac evaluate_fp_opts_unchanged \\ fs[]
+    \\ imp_res_tac evaluate_fp_opts_fixed \\ fs[]
     (*
     \\ qmatch_goalsub_abbrev_tac`evaluate_match t1`
     \\ first_x_assum(qspec_then`t1`mp_tac)
@@ -930,7 +905,7 @@ Proof
       \\ qmatch_goalsub_abbrev_tac`evaluate t1 _ [_]`
       \\ first_x_assum(qspec_then`t1`mp_tac)
       \\ fs[Abbr`t1`]
-      \\ imp_res_tac evaluate_fp_opts_unchanged
+      \\ imp_res_tac evaluate_fp_opts_fixed
       \\ imp_res_tac evaluate_state_const \\ fs[])
     \\ TOP_CASE_TAC \\ fs[]
     >- (
@@ -951,7 +926,7 @@ Proof
     >- (
       rpt strip_tac  \\ rveq \\ fs[]
       \\ TOP_CASE_TAC \\ fs[]
-      \\ reverse TOP_CASE_TAC \\ fs[]
+      \\ reverse TOP_CASE_TAC \\ fs[shift_fp_opts_def]
       \\ `q.ffi = s.ffi`
         by (rveq
         \\ imp_res_tac do_app_io_events_mono
@@ -962,20 +937,20 @@ Proof
       \\ rveq \\ fs[]
       \\ imp_res_tac fpOp_determ \\ fs[]
       \\ rveq \\ fs[state_component_equality]
-      \\ imp_res_tac evaluate_fp_opts_unchanged \\ rveq \\ fs[])
-    \\ rpt strip_tac \\ rveq \\ fs[]
+      \\ imp_res_tac evaluate_fp_opts_fixed \\ rveq \\ fs[])
+    \\ rpt strip_tac \\ rveq \\ fs[shift_fp_opts_def]
     \\ rveq
     \\ imp_res_tac do_app_io_events_mono
     \\ imp_res_tac evaluate_io_events_mono_imp
     \\ imp_res_tac io_events_mono_antisym \\ fs[]
     \\ imp_res_tac do_app_SOME_ffi_same \\ fs[]
-    \\ res_tac
     \\ `! outcome. r' <> Rerr (Rabort (Rffi_error outcome))`
         by (rpt strip_tac \\ rveq \\ fs[do_fprw_def])
     \\ res_tac
     \\ first_x_assum (qspec_then `t.ffi` assume_tac)
     \\ fs[]
-    \\ imp_res_tac evaluate_fp_opts_unchanged \\ fs[state_component_equality])
+    \\ imp_res_tac evaluate_fp_opts_fixed
+    \\ first_x_assum drule\\ fs[state_component_equality])
   >- (
     rfs[evaluate_def]
     \\ qpat_x_assum`_ = (_,_)`mp_tac
@@ -989,7 +964,7 @@ Proof
     \\ rename1`evaluate s _ _ = (s1,_)`
     \\ `s1.ffi = s.ffi` by metis_tac[evaluate_ffi_sandwich]
     \\ fs[] \\ rfs[]
-    \\ imp_res_tac evaluate_fp_opts_unchanged
+    \\ imp_res_tac evaluate_fp_opts_fixed
     \\ qmatch_goalsub_abbrev_tac`evaluate t1 _ [_]`
     \\ first_x_assum(qspec_then`t1`mp_tac)
     \\ simp[Abbr`t1`]
@@ -1006,7 +981,7 @@ Proof
     \\ rename1`evaluate s _ _ = (s1,_)`
     \\ `s1.ffi = s.ffi` by metis_tac[evaluate_ffi_sandwich]
     \\ fs[] \\ rfs[]
-    \\ imp_res_tac evaluate_fp_opts_unchanged
+    \\ imp_res_tac evaluate_fp_opts_fixed
     \\ qmatch_goalsub_abbrev_tac`evaluate t1 _ [_]`
     \\ first_x_assum(qspec_then`t1`mp_tac)
     \\ simp[Abbr`t1`]
@@ -1022,7 +997,7 @@ Proof
     \\ rename1`evaluate s _ _ = (s1,_)`
     \\ `s1.ffi = s.ffi` by metis_tac[evaluate_match_ffi_sandwich]
     \\ fs[] \\ rfs[]
-    \\ imp_res_tac evaluate_fp_opts_unchanged
+    \\ imp_res_tac evaluate_fp_opts_fixed
     \\ qmatch_goalsub_abbrev_tac`evaluate_match t1`
     \\ first_x_assum(qspec_then`t1`mp_tac)
     \\ simp[Abbr`t1`]
@@ -1038,7 +1013,7 @@ Proof
     \\ rename1`evaluate s _ _ = (s1,_)`
     \\ `s1.ffi = s.ffi` by metis_tac[evaluate_ffi_sandwich]
     \\ fs[] \\ rfs[]
-    \\ imp_res_tac evaluate_fp_opts_unchanged
+    \\ imp_res_tac evaluate_fp_opts_fixed
     \\ qmatch_goalsub_abbrev_tac`evaluate t1 _ [_]`
     \\ first_x_assum(qspec_then`t1`mp_tac)
     \\ simp[Abbr`t1`]
