semantics/proofs/fpSemPropsScript.sml
@@ -2,11 +2,67 @@
   Properties of floating-point value tree semantics
 *)
 
-open preamble fpSemTheory fpValTreeTheory semanticPrimitivesTheory;
+open preamble fpSemTheory fpValTreeTheory semanticPrimitivesTheory evaluateTheory;
 open terminationTheory;
 
 val _ = new_theory "fpSemProps";
 
+Theorem fp_opts_mono[local]:
+  ! (s1 s2 s3:'a state) n m.
+    (! x. s1.fp_opts (n + x) = s2.fp_opts x) /\
+    (! x. s2.fp_opts (m + x) = s3.fp_opts x) ==>
+    ? k. ! x. s1.fp_opts (k + x) = s3.fp_opts x
+Proof
+  rpt strip_tac \\ qexists_tac `n+m`
+  \\ qpat_x_assum `! x. _ _ = s3.fp_opts _` (qspec_then `x` (fn thm => fs[GSYM thm]))
+  \\ qpat_x_assum `! x. _ _ = s2.fp_opts _` (qspec_then `m + x` (fn thm => fs[GSYM thm]))
+QED
+
+Theorem fp_opts_add_1[local]:
+  ! (s1 s2:'a state) n m.
+    (! x. s1.fp_opts (n + x) = s2.fp_opts x) ==>
+    ? k. ! x. s1.fp_opts (k + x) = s2.fp_opts (x + 1)
+Proof
+  rpt strip_tac
+  \\ qexists_tac `n+1` \\ fs[]
+QED
+
+Theorem evaluate_fp_opts_fixed:
+  (! (s:'a state) env e s' r.
+    evaluate s env e = (s', r) ==>
+    (?n. ! x. s.fp_opts (x + n) = s'.fp_opts x) /\
+    s.fp_rws = s'.fp_rws) /\
+  (! (s:'a state) env v pes errv s' r.
+    evaluate_match s env v pes errv = (s', r) ==>
+    (?n. ! x. s.fp_opts (x + n) = s'.fp_opts x) /\
+    s.fp_rws = s'.fp_rws)
+Proof
+  ho_match_mp_tac evaluate_ind \\ rw[]
+  \\ rfs[evaluate_def] \\ rveq
+  \\ TRY (qexists_tac `0` \\ fs[] \\ NO_TAC)
+  \\ qpat_x_assum `_ = (_,_)` mp_tac
+  \\ rpt (TOP_CASE_TAC \\ fs[])
+  \\ rpt strip_tac \\ rveq
+  \\ res_tac \\ fs[dec_clock_def, shift_fp_opts_def]
+  \\ imp_res_tac fp_opts_mono
+  \\ imp_res_tac fp_opts_add_1
+  \\ TRY (asm_exists_tac \\ fs[])
+  \\ qexists_tac `0` \\ fs[]
+QED
+
+Theorem fpOp_determ:
+  ! op refs refsN (ffi1 ffi1':'a ffi_state) (ffi2:'b ffi_state) r vl.
+    isFpOp op /\
+    do_app (refs, ffi1) op vl = SOME ((refsN, ffi1'), r) ==>
+    do_app (refs, ffi2) op vl = SOME ((refsN, ffi2), r)
+Proof
+  rpt strip_tac \\ Cases_on `op` \\ fs[astTheory.isFpOp_def]
+  \\ rpt (qpat_x_assum `do_app _ _ _ = _` mp_tac)
+  \\ fs[do_app_def]
+  \\ rpt (TOP_CASE_TAC \\ fs[])
+QED
+
+(*
 Theorem compress_word_valid:
   ! v.
     isFpWordOp v ==>
@@ -27,5 +83,6 @@ Proof
   \\ rename [`fp_cmp_comp f1 w1 w2`]
   \\ qexists_tac `fp_cmp_comp f1 w1 w2` \\ fs[]
 QED
+*)
 
 val _ = export_theory();
